remove three admits in poly1305

code/poly1305/Hacl.Impl.Poly1305.Field32xN.fst
@@ -815,124 +815,57 @@ let load_felem_le #w f b =
   LSeq.eq_intro (feval h1 f) (LSeq.create w (BSeq.nat_from_bytes_le (as_seq h0 b)))
 
 inline_for_extraction noextract
-val bytes_to_limbs:
-    #w:lanes
-  -> b:lbuffer uint8 16ul
-  -> Stack (uint64xN w & uint64xN w)
+val uints64_from_bytes_le:
+    b:lbuffer uint8 16ul
+  -> Stack (uint64 & uint64)
     (requires fun h -> live h b)
     (ensures  fun h0 (lo, hi) h1 -> h0 == h1 /\
-     (forall (i:nat). i < w ==>
-       (uint64xN_v hi).[i] * pow2 64 + (uint64xN_v lo).[i] ==
-       BSeq.nat_from_bytes_le (as_seq h0 b)))
-let bytes_to_limbs #w b =
+      v hi * pow2 64 + v lo == BSeq.nat_from_bytes_le (as_seq h0 b))
+let uints64_from_bytes_le b =
   let h0 = ST.get () in
   let lo = uint_from_bytes_le #U64 (sub b 0ul 8ul) in
   let hi = uint_from_bytes_le #U64 (sub b 8ul 8ul) in
-  let f0 = vec_load lo w in
-  let f1 = vec_load hi w in
   uint_from_bytes_le_lemma (as_seq h0 b);
-  f0, f1
+  lo, hi
 
 inline_for_extraction noextract
-val store_felem:
+val uints64_from_felem_le:
     #w:lanes
   -> f:felem w
-  -> Stack (uint64xN w & uint64xN w)
+  -> Stack (uint64 & uint64)
     (requires fun h ->
       live h f /\ felem_fits h f (1, 1, 1, 1, 1))
     (ensures  fun h0 (lo, hi) h1 -> h0 == h1 /\
-      (forall (i:nat). i < w ==>
-	(uint64xN_v hi).[i] * pow2 64 + (uint64xN_v lo).[i] == (fas_nat h0 f).[i] % pow2 128))
-let store_felem #w f =
-  let f0 = f.(0ul) in
-  let f1 = f.(1ul) in
-  let f2 = f.(2ul) in
-  let f3 = f.(3ul) in
-  let f4 = f.(4ul) in
+      v hi * pow2 64 + v lo == (fas_nat h0 f).[0] % pow2 128)
+let uints64_from_felem_le #w f =
+  let (f0, f1, f2, f3, f4) = (f.(0ul), f.(1ul), f.(2ul), f.(3ul), f.(4ul)) in
   store_felem5 #w (f0, f1, f2, f3, f4)
 
 inline_for_extraction noextract
-val store_felem1_le:
+val uints64_to_bytes_le:
     b:lbuffer uint8 16ul
-  -> lo:uint64xN 1
-  -> hi:uint64xN 1
+  -> lo:uint64
+  -> hi:uint64
   -> Stack unit
     (requires fun h -> live h b)
     (ensures  fun h0 _ h1 ->
       modifies (loc b) h0 h1 /\
-      as_seq h1 b == BSeq.nat_to_bytes_le 16 ((uint64xN_v hi).[0] * pow2 64 + (uint64xN_v lo).[0]))
-let store_felem1_le b r0 r1 =
+      as_seq h1 b == BSeq.nat_to_bytes_le 16 (v hi * pow2 64 + v lo))
+let uints64_to_bytes_le b r0 r1 =
   let h0 = ST.get () in
-  vec_store_le (sub b 0ul 8ul) r0;
-  vec_store_le (sub b 8ul 8ul) r1;
+  update_sub_f h0 b 0ul 8ul
+    (fun h -> BSeq.uint_to_bytes_le #U64 r0)
+    (fun _ -> uint_to_bytes_le (sub b 0ul 8ul) r0);
   let h1 = ST.get () in
-  uints_to_bytes_le_lemma64_1 (vec_v r0) (vec_v r1);
-  LSeq.lemma_concat2 8 (LSeq.sub (as_seq h1 b) 0 8) 8 (LSeq.sub (as_seq h1 b) 8 8) (as_seq h1 b)
-
-inline_for_extraction noextract
-val store_felem2_le:
-    b:lbuffer uint8 16ul
-  -> lo:uint64xN 2
-  -> hi:uint64xN 2
-  -> Stack unit
-    (requires fun h -> live h b)
-    (ensures  fun h0 _ h1 ->
-      modifies (loc b) h0 h1 /\
-      as_seq h1 b == BSeq.nat_to_bytes_le 16 ((uint64xN_v hi).[0] * pow2 64 + (uint64xN_v lo).[0]))
-let store_felem2_le b f0 f1 =
-  let r0 = vec_interleave_low f0 f1 in
-  vec_interleave_low_lemma2 f0 f1;
-  vec_store_le b r0;
-  uints_to_bytes_le_lemma64_2 (vec_v r0)
-
-inline_for_extraction noextract
-val store_felem4_le:
-    b:lbuffer uint8 16ul
-  -> lo:uint64xN 4
-  -> hi:uint64xN 4
-  -> Stack unit
-    (requires fun h -> live h b)
-    (ensures  fun h0 _ h1 ->
-      modifies (loc b) h0 h1 /\
-      as_seq h1 b == BSeq.nat_to_bytes_le 16 ((uint64xN_v hi).[0] * pow2 64 + (uint64xN_v lo).[0]))
-let store_felem4_le b f0 f1 =
-  push_frame ();
-  let lo = vec_interleave_low f0 f1 in
-  let hi = vec_interleave_high f0 f1 in
-  vec_interleave_low_lemma_uint64_4 f0 f1;
-  vec_interleave_high_lemma_uint64_4 f0 f1;  let lo1 = cast U128 2 lo in
-  let hi1 = cast U128 2 hi in
-  lemma_cast_vec64_to_vec128 lo;
-  lemma_cast_vec64_to_vec128 hi;
-  let r0 = vec_interleave_low lo1 hi1 in
-  vec_interleave_low_lemma2 lo1 hi1;
-  let tmp = create 32ul (u8 0) in
-  vec_store_le tmp r0;
-  uints_to_bytes_le_lemma128_2 (vec_v r0);
-  let h0 = ST.get () in
-  copy b (sub tmp 0ul 16ul);
-  let h1 = ST.get () in
-  assert (as_seq h1 b == BSeq.uint_to_bytes_le (vec_v r0).[0]);
-  assert (v (vec_v r0).[0] == v (vec_v f1).[0] * pow2 64 + v (vec_v f0).[0]);
-  uint_to_bytes_le_lemma128 (vec_v r0).[0];
-  pop_frame()
-
-inline_for_extraction noextract
-val store_felem_le:
-    #w:lanes
-  -> b:lbuffer uint8 16ul
-  -> lo:uint64xN w
-  -> hi:uint64xN w
-  -> Stack unit
-    (requires fun h -> live h b)
-    (ensures  fun h0 _ h1 ->
-      modifies (loc b) h0 h1 /\
-      as_seq h1 b == BSeq.nat_to_bytes_le 16 ((uint64xN_v hi).[0] * pow2 64 + (uint64xN_v lo).[0]))
-let store_felem_le #w b lo hi =
-  match w with
-  | 1 -> store_felem1_le b lo hi
-  | 2 -> store_felem2_le b lo hi
-  | 4 -> store_felem4_le b lo hi
+  update_sub_f h1 b 8ul 8ul
+    (fun h -> BSeq.uint_to_bytes_le #U64 r1)
+    (fun _ -> uint_to_bytes_le (sub b 8ul 8ul) r1);
+  //uint_to_bytes_le (sub b 0ul 8ul) r0;
+  //uint_to_bytes_le (sub b 8ul 8ul) r1;
+  let h2 = ST.get () in
+  uints64_to_bytes_le_lemma r0 r1;
+  LSeq.eq_intro (LSeq.sub (as_seq h2 b) 0 8) (BSeq.uint_to_bytes_le #U64 r0);
+  LSeq.lemma_concat2 8 (BSeq.uint_to_bytes_le #U64 r0) 8 (BSeq.uint_to_bytes_le #U64 r1) (as_seq h2 b)
 
 //inline_for_extraction noextract
 [@CInline]
@@ -1075,20 +1008,13 @@ let fmul_rn_normalize #w out p =
 
 inline_for_extraction noextract
 val mod_add128:
-    #w:lanes
-  -> a:(uint64xN w & uint64xN w)
-  -> b:(uint64xN w & uint64xN w)
-  -> Pure (uint64xN w & uint64xN w)
+    a:(uint64 & uint64)
+  -> b:(uint64 & uint64)
+  -> Pure (uint64 & uint64)
     (requires True)
     (ensures (fun (r0, r1) ->
-      let (a0, a1) = a in
-      let (b0, b1) = b in
-      (uint64xN_v r1).[0] * pow2 64 + (uint64xN_v r0).[0] ==
-	(((uint64xN_v a1).[0] + (uint64xN_v b1).[0]) * pow2 64 + (uint64xN_v a0).[0] + (uint64xN_v b0).[0]) % pow2 128))
-let mod_add128 #w (a0, a1) (b0, b1) =
-  let r0 = vec_add_mod a0 b0 in
-  let r1 = vec_add_mod a1 b1 in
-  let c = r0 ^| ((r0 ^| b0) `vec_or` ((r0 -| b0) ^| b0)) >>| 63ul in
-  let r1 = vec_add_mod r1 c in
+      let (a0, a1) = a in let (b0, b1) = b in
+      v r1 * pow2 64 + v r0 == ((v a1 + v b1) * pow2 64 + v a0 + v b0) % pow2 128))
+let mod_add128 (a0, a1) (b0, b1) =
   mod_add128_lemma (a0, a1) (b0, b1);
-  (r0, r1)
+  mod_add128 (a0, a1) (b0, b1)
